src/Examples/Interprocedural/Example_Side_Execute.thy
@@ -22,18 +22,18 @@ text \<open>
   evaluate at build time): \<open>x\<close> is \<open>SPos\<close>, an untouched \<open>y\<close> stays \<open>STop\<close>.
 \<close>
 
-value "sign_exec_prog x1_prog ''x''"
-value "sign_exec_prog x1_prog ''y''"
+value "sign_exec_prog ''main'' x1_prog ''x''"
+value "sign_exec_prog ''main'' x1_prog ''y''"
 
 text \<open>The solver computes \<open>x \<mapsto> SPos\<close> at the exit, captured as a theorem
   by code reflection.\<close>
 
 lemma x1_computes_x_pos:
-  "sign_exec_prog x1_prog ''x'' = SPos"
+  "sign_exec_prog ''main'' x1_prog ''x'' = SPos"
   by eval
 
 lemma x1_y_top:
-  "sign_exec_prog x1_prog ''y'' = STop"
+  "sign_exec_prog ''main'' x1_prog ''y'' = STop"
   by eval
 
 text \<open>
@@ -42,7 +42,7 @@ text \<open>
   @{thm sign_terminates_prog_via_solve_c} the program lies in the solver's domain.
 \<close>
 
-lemma x1_terminates: "sign_terminates_prog x1_prog"
+lemma x1_terminates: "sign_terminates_prog ''main'' x1_prog"
   by (rule sign_terminates_prog_via_solve_c) eval
 
 text \<open>
@@ -53,8 +53,8 @@ text \<open>
 \<close>
 
 corollary x1_certified_sound:
-  "ltr_collect (prog_cfg x1_prog) cinit_stores (cfg_exit (prog_cfg x1_prog))
-   \<le> \<lbrakk>sign_exec_prog x1_prog\<rbrakk>"
+  "ltr_collect (prog_cfg ''main'' x1_prog) cinit_stores (cfg_exit (prog_cfg ''main'' x1_prog))
+   \<le> \<lbrakk>sign_exec_prog ''main'' x1_prog\<rbrakk>"
   by (rule sign_exec_prog_sound_collecting[OF x1_terminates])
 
 definition x1_s0 :: store where
@@ -71,9 +71,9 @@ lemma x1_completed:
 
 lemma x1_completed_run_collect:
   "x1_s0(''x'' := 1) \<in>
-    ltr_collect (compile_prog (prog_table x1_prog) (prog_procs x1_prog) (prog_main x1_prog))
+    ltr_collect (compile_prog (prog_table x1_prog) (prog_procs x1_prog) ''main'' (prog_main x1_prog))
       cinit_stores
-      (cfg_exit (compile_prog (prog_table x1_prog) (prog_procs x1_prog) (prog_main x1_prog)))"
+      (cfg_exit (compile_prog (prog_table x1_prog) (prog_procs x1_prog) ''main'' (prog_main x1_prog)))"
 proof -
   have init: "x1_s0 \<in> cinit_stores"
     by (simp add: x1_s0_def cinit_stores_def)
@@ -94,7 +94,7 @@ qed
 theorem x1_explicit_completed_run_covered:
   "pcompletes (prog_table x1_prog) (prog_main x1_prog) x1_s0
       (x1_s0(''x'' := 1))
-   \<and> x1_s0(''x'' := 1) \<in> \<lbrakk>sign_exec_prog x1_prog\<rbrakk>"
+   \<and> x1_s0(''x'' := 1) \<in> \<lbrakk>sign_exec_prog ''main'' x1_prog\<rbrakk>"
 proof
   show "pcompletes (prog_table x1_prog) (prog_main x1_prog) x1_s0
       (x1_s0(''x'' := 1))"
@@ -102,10 +102,10 @@ proof
 next
   have collect:
     "x1_s0(''x'' := 1) \<in>
-      ltr_collect (prog_cfg x1_prog) cinit_stores (cfg_exit (prog_cfg x1_prog))"
+      ltr_collect (prog_cfg ''main'' x1_prog) cinit_stores (cfg_exit (prog_cfg ''main'' x1_prog))"
     using x1_completed_run_collect
     by (simp add: prog_cfg_def)
-  show "x1_s0(''x'' := 1) \<in> \<lbrakk>sign_exec_prog x1_prog\<rbrakk>"
+  show "x1_s0(''x'' := 1) \<in> \<lbrakk>sign_exec_prog ''main'' x1_prog\<rbrakk>"
     using x1_certified_sound collect by blast
 qed
 
@@ -121,4 +121,6 @@ ML_val \<open>
 \<close>
 
 end
+
+
 
