src/Examples/Interprocedural/Example_Side_Proc_Global.thy
@@ -41,7 +41,7 @@ theorem proc_global_side_sign_analysis:
     "side_cfg_solve_dom_eff (compile_prog inc_pi [''p''] ''main'' (imp \<lbrakk> p() \<rbrakk>)) sign_etf bot
        side_proc_global_s0 ()
        (cfg_exit (compile_prog inc_pi [''p''] ''main'' (imp \<lbrakk> p() \<rbrakk>)))"
-  shows "t \<in> \<lbrakk>side_analyse_eff inc_pi [''p''] (imp \<lbrakk> p() \<rbrakk>) sign_etf bot side_proc_global_s0 ()
+  shows "t \<in> \<lbrakk>side_analyse_eff inc_pi [''p''] ''main'' (imp \<lbrakk> p() \<rbrakk>) sign_etf bot side_proc_global_s0 ()
          (cfg_exit (compile_prog inc_pi [''p''] ''main'' (imp \<lbrakk> p() \<rbrakk>)))\<rbrakk>"
   by (rule side_sign_analysis_sound[OF s_sound collect_exit side_solve_dom])
 subsection \<open>Executable sign analysis\<close>
@@ -56,18 +56,18 @@ definition inc_prog :: imp_prog where
   "inc_prog = imp_prog.make [(''p'', the (inc_pi ''p''))] inc_main"
 
 
-value "sign_exec_prog inc_prog ''Gx''"
+value "sign_exec_prog ''main'' inc_prog ''Gx''"
 
 lemma inc_gx_nonneg:
-  "sign_exec_prog inc_prog ''Gx'' = SNonNeg"
+  "sign_exec_prog ''main'' inc_prog ''Gx'' = SNonNeg"
   by eval
 
-lemma inc_terminates: "sign_terminates_prog inc_prog"
+lemma inc_terminates: "sign_terminates_prog ''main'' inc_prog"
   by (rule sign_terminates_prog_via_solve_c) eval
 
 corollary inc_certified_sound:
-  "ltr_collect (prog_cfg inc_prog) cinit_stores (cfg_exit (prog_cfg inc_prog))
-   \<le> \<lbrakk>sign_exec_prog inc_prog\<rbrakk>"
+  "ltr_collect (prog_cfg ''main'' inc_prog) cinit_stores (cfg_exit (prog_cfg ''main'' inc_prog))
+   \<le> \<lbrakk>sign_exec_prog ''main'' inc_prog\<rbrakk>"
   by (rule sign_exec_prog_sound_collecting[OF inc_terminates])
 
 subsection \<open>Annotated CFG visualisation\<close>
@@ -83,4 +83,6 @@ ML_val \<open>
 \<close>
 
 end
+
+
 
